Tl_bisim is an equivalence relation
We prove the preceding statement. This allows us to complete the proof
that equality of trace languages (rather than just bisimilarity) also
implies equivalence of the underlying session types.

src/TLFacts.v
@@ -3,6 +3,78 @@ Require Import Contractive Env Free FreeFacts Map Msg Sty Shape
 Require Import FunctionalExtensionality.
 
 
+(******************************************************************************)
+(* Facts about Tl_bisim *)
+
+
+Inductive R_Tl_bisim_reflexive : Tl -> Tl -> Prop :=
+| R_Tl_bisim_reflexive_intro :
+    forall l,
+    R_Tl_bisim_reflexive l l
+.
+
+Lemma Tl_bisim_reflexive :
+  forall l,
+  Tl_bisim l l.
+Proof.
+  intros. apply Tl_bisim_coind with (R := R_Tl_bisim_reflexive);
+    [|constructor; auto].
+  clear. introv H. inverts H. rename l' into l. destruct l; constructor;
+    constructor.
+Qed.
+
+
+Inductive R_Tl_bisim_symmetric : Tl -> Tl -> Prop :=
+| R_Tl_bisim_symmetric_intro :
+    forall l l',
+    Tl_bisim l l' ->
+    R_Tl_bisim_symmetric l' l
+.
+
+Lemma Tl_bisim_symmetric :
+  forall l l',
+  Tl_bisim l l' ->
+  Tl_bisim l' l.
+Proof.
+  intros. apply Tl_bisim_coind with (R := R_Tl_bisim_symmetric);
+    [|constructor; auto].
+  clear. introv H. inverts1 H. inverts2 H; constructor; constructor; auto.
+Qed.
+
+
+
+Inductive R_Tl_bisim_transitive : Tl -> Tl -> Prop :=
+| R_Tl_bisim_transitive_intro :
+    forall l1 l2 l3,
+    Tl_bisim l1 l2 ->
+    Tl_bisim l2 l3 ->
+    R_Tl_bisim_transitive l1 l3
+.
+
+Lemma Tl_bisim_transitive :
+  forall l1 l2 l3,
+  Tl_bisim l1 l2 ->
+  Tl_bisim l2 l3 ->
+  Tl_bisim l1 l3.
+Proof.
+  intros. apply Tl_bisim_coind with (R := R_Tl_bisim_transitive);
+    [|econstructor; eauto].
+  clear. introv H. inversion_clear H as [l1 l2 l3 H1 H2]. subst.
+  inverts2 H1; inverts2 H2; constructor; econstructor; eauto.
+Qed.
+
+
+Add Relation Tl Tl_bisim
+  reflexivity proved by Tl_bisim_reflexive
+  symmetry proved by Tl_bisim_symmetric
+  transitivity proved by Tl_bisim_transitive
+  as Tl_bisim_rel.
+
+
+(******************************************************************************)
+(* Facts about tl *)
+
+
 Lemma tl_contractive_irrelevant :
   forall eta S contr contr',
   tl eta S contr = tl eta S contr'.
